Working on proof and adding notes

x86/proofs/mldsa_mont_mul.ml
@@ -14,8 +14,11 @@ loadt "x86/proofs/base.ml";;
 (* Working Proof *)
 needs "x86/proofs/base.ml";;
 
-(*
- # print_literal_from_elf "x86/mldsa/mldsa_mont_mul.o";;
+(* We are taking 9 instructions from within the mldsa NTT.
+https://github.com/pq-code-package/mldsa-native/blob/main/mldsa/native/x86_64/src/ntt.S#L36-L48 *)
+
+(* 
+# print_literal_from_elf "x86/mldsa/mldsa_mont_mul.o";;
 [
   0xc4; 0x42; 0x75; 0x28; 0xe8;         (* VPMULDQ (%_% ymm13) (%_% ymm1) (%_% ymm8) *)                  
   0xc4; 0x41; 0x7e; 0x16; 0xe0;         (* VMOVSHDUP (%_% ymm12) (%_% ymm8) *)               
@@ -25,12 +28,13 @@ needs "x86/proofs/base.ml";;
   0xc4; 0x42; 0x7d; 0x28; 0xed;         (* VPMULDQ (%_% ymm13) (%_% ymm0) (%_% ymm13) *)      
   0xc4; 0x42; 0x7d; 0x28; 0xf6;         (* VPMULDQ (%_% ymm14) (%_% ymm0) (%_% ymm14) *)
   0xc4; 0x41; 0x7e; 0x16; 0xc0;         (* VMOVSHDUP (%_% ymm8) (%_% ymm8) *)      
-  0xc4; 0x43; 0x3d; 0x02; 0xc4; 0xaa;   (* VPBLENDD (%_% ymm8) (%_% ymm8) (%_% ymm12) (Imm8 (word 170)) *)             
-  0xc3                                  (* RET *)
+  0xc4; 0x43; 0x3d; 0x02; 0xc4; 0xaa;   (* VPBLENDD (%_% ymm8) (%_% ymm8) (%_% ymm12) (Imm8 (word 170)) *)
 ];;
  *)
 
-(*
+
+(* A description of these 9 instructions is as follows:
+
 # Montgomery multiplication: h * zeta -> t (instructions 1-9)
 vpmuldq    %ymm1,%ymm8,%ymm13          # h * zeta_low -> ymm13
 vmovshdup  %ymm8,%ymm12                # extract high parts of h
@@ -63,7 +67,6 @@ let mldsa_mont_mul = define_assert_from_elf "mldsa_mont_mul" "x86/mldsa/mldsa_mo
                            (* VMOVSHDUP (%_% ymm8) (%_% ymm8) *)
   0xc4; 0x43; 0x3d; 0x02; 0xc4; 0xaa;
                            (* VPBLENDD (%_% ymm8) (%_% ymm8) (%_% ymm12) (Imm8 (word 170)) *)
-  0xc3                     (* RET *)
 ];;
 
 (* 
@@ -75,14 +78,14 @@ val mldsa_mont_mul : thm =
       word 66; word 109; word 40; word 228; word 196; word 66; word 125;
       word 40; word 237; word 196; word 66; word 125; word 40; word 246;
       word 196; word 65; word 126; word 22; word 192; word 196; word 67;
-      word 61; word 2; word 196; word 170; word 195]
+      word 61; word 2; word 196; word 170]
 *)
 
 let EXEC = X86_MK_EXEC_RULE mldsa_mont_mul;;
-
+let EXEC_length, EXEC_contents = EXEC;;
 (* 
 val EXEC : thm * thm option array =
-  (|- LENGTH mldsa_mont_mul = 47,
+  (|- LENGTH mldsa_mont_mul = 46,
    [|Some
       |- forall s pc.
              bytes_loaded s (word pc) mldsa_mont_mul
@@ -138,12 +141,10 @@ val EXEC : thm * thm option array =
                  (6,
                   VPBLENDD (%_% ymm8) (%_% ymm8) (%_% ymm12)
                   (Imm8 (word 170)));
-     None; None; None; None; None;
-     Some
-      |- forall s pc.
-             bytes_loaded s (word pc) mldsa_mont_mul
-             ==> x86_decode s (word (pc + 46)) (1,RET)|])
+     None; None; None; None; None|])
 *)
+
+(* Specifications *)
 
 let MLDSA_MONT_MUL_SPEC = prove(
   `forall pc h zeta qinv zeta_high.
@@ -154,12 +155,2033 @@ let MLDSA_MONT_MUL_SPEC = prove(
          read YMM1 s = zeta /\
          read YMM2 s = zeta_high /\
          read YMM8 s = h)
-    (\s. read RIP s = word (pc + 47) /\ T)
+    (\s. read RIP s = word (pc + 46))
     (MAYCHANGE [RIP] ,, MAYCHANGE [YMM8; YMM12; YMM13; YMM14] ,, MAYCHANGE SOME_FLAGS)`,
 
   REPEAT STRIP_TAC THEN
   REWRITE_TAC [SOME_FLAGS; fst EXEC] THEN
   ENSURES_INIT_TAC "s0" THEN
-  X86_STEPS_TAC EXEC (1--10) THEN
+  X86_STEPS_TAC EXEC (1--9) THEN
   ENSURES_FINAL_STATE_TAC THEN
   ASM_REWRITE_TAC[]);;
+
+(* Output from stepping each part in Hol-light REPL server (while working on proof) *)
+
+(* Set current term as goal:
+`forall pc h zeta qinv zeta_high.
+     ensures x86
+     (\s.
+          bytes_loaded s (word pc) mldsa_mont_mul /\
+          read RIP s = word pc /\
+          read YMM0 s = qinv /\
+          read YMM1 s = zeta /\
+          read YMM2 s = zeta_high /\
+          read YMM8 s = h)
+     (\s. read RIP s = word (pc + 46))
+     (MAYCHANGE [RIP] ,,
+      MAYCHANGE [YMM8; YMM12; YMM13; YMM14] ,,
+      MAYCHANGE SOME_FLAGS)`
+*)
+
+(* Output:
+`forall pc h zeta qinv zeta_high.
+     ensures x86
+     (\s.
+          bytes_loaded s (word pc) mldsa_mont_mul /\
+          read RIP s = word pc /\
+          read YMM0 s = qinv /\
+          read YMM1 s = zeta /\
+          read YMM2 s = zeta_high /\
+          read YMM8 s = h)
+     (\s. true)
+     (MAYCHANGE [RIP] ,,
+      MAYCHANGE [YMM8; YMM12; YMM13; YMM14] ,,
+      MAYCHANGE SOME_FLAGS)`
+*)
+
+
+(* Execute current tatic: REPEAT STRIP_TAC *)
+(* Output:
+`ensures x86
+ (\s.
+      bytes_loaded s (word pc) mldsa_mont_mul /\
+      read RIP s = word pc /\
+      read YMM0 s = qinv /\
+      read YMM1 s = zeta /\
+      read YMM2 s = zeta_high /\
+      read YMM8 s = h)
+ (\s. read RIP s = word (pc + 46))
+ (MAYCHANGE [RIP] ,,
+  MAYCHANGE [YMM8; YMM12; YMM13; YMM14] ,,
+  MAYCHANGE SOME_FLAGS)`
+*)
+
+(* Execute current tatic: REWRITE_TAC [SOME_FLAGS; fst EXEC]  *)
+(* Output:
+`ensures x86
+ (\s.
+      bytes_loaded s (word pc) mldsa_mont_mul /\
+      read RIP s = word pc /\
+      read YMM0 s = qinv /\
+      read YMM1 s = zeta /\
+      read YMM2 s = zeta_high /\
+      read YMM8 s = h)
+ (\s. read RIP s = word (pc + 46))
+ (MAYCHANGE [RIP] ,,
+  MAYCHANGE [YMM8; YMM12; YMM13; YMM14] ,,
+  MAYCHANGE [CF; PF; AF; ZF; SF; OF])`
+*)
+
+(* Execute current tatic: ENSURES_INIT_TAC "s0"  *)
+(* Output:
+val it : goalstack = 1 subgoal (1 total)
+
+  0 [`bytes_loaded s0 (word pc) mldsa_mont_mul`]
+  1 [`read RIP s0 = word pc`]
+  2 [`read YMM0 s0 = qinv`]
+  3 [`read YMM1 s0 = zeta`]
+  4 [`read YMM2 s0 = zeta_high`]
+  5 [`read YMM8 s0 = h`]
+  6 [`(MAYCHANGE:((x86state,?272209)component)list->x86state->x86state->bool)
+      []
+      s0
+      s0`]
+
+`eventually x86
+ (\s'.
+      read RIP s' = word (pc + 46) /\
+      (MAYCHANGE [RIP] ,,
+       MAYCHANGE [YMM8; YMM12; YMM13; YMM14] ,,
+       MAYCHANGE [CF; PF; AF; ZF; SF; OF])
+      s0
+      s')
+ s0`
+*)
+
+(* Execute current tatic: X86_STEPS_TAC EXEC (1--9) *)
+(* Output:
+Stepping to state s1
+CPU time (user): 0.160738
+Stepping to state s2
+CPU time (user): 0.133099
+Stepping to state s3
+CPU time (user): 0.191659
+Stepping to state s4
+CPU time (user): 0.173835
+Stepping to state s5
+CPU time (user): 0.20204
+Stepping to state s6
+CPU time (user): 0.220225
+Stepping to state s7
+CPU time (user): 0.328331
+Stepping to state s8
+CPU time (user): 0.245162
+Stepping to state s9
+CPU time (user): 0.266097
+val it : goalstack = 1 subgoal (1 total)
+
+  0 [`bytes_loaded s9 (word pc) mldsa_mont_mul`]
+  1 [`read YMM13 s9 =
+      word_join
+      (word_join
+       (word_mul (word_sx (word_subword (word_subword qinv (192,64)) (0,32)))
+       (word_sx
+       (word_subword
+        (word_subword
+         (word_join
+          (word_join
+           (word_mul
+            (word_sx (word_subword (word_subword zeta (192,64)) (0,32)))
+           (word_sx (word_subword (word_subword h (192,64)) (0,32))))
+          (word_mul
+           (word_sx (word_subword (word_subword zeta (128,64)) (0,32)))
+          (word_sx (word_subword (word_subword h (128,64)) (0,32)))))
+         (word_join
+          (word_mul
+           (word_sx (word_subword (word_subword zeta (64,64)) (0,32)))
+          (word_sx (word_subword (word_subword h (64,64)) (0,32))))
+         (word_mul (word_sx (word_subword (word_subword zeta (0,64)) (0,32)))
+         (word_sx (word_subword (word_subword h (0,64)) (0,32))))))
+        (192,64))
+       (0,32))))
+      (word_mul (word_sx (word_subword (word_subword qinv (128,64)) (0,32)))
+      (word_sx
+      (word_subword
+       (word_subword
+        (word_join
+         (word_join
+          (word_mul
+           (word_sx (word_subword (word_subword zeta (192,64)) (0,32)))
+          (word_sx (word_subword (word_subword h (192,64)) (0,32))))
+         (word_mul
+          (word_sx (word_subword (word_subword zeta (128,64)) (0,32)))
+         (word_sx (word_subword (word_subword h (128,64)) (0,32)))))
+        (word_join
+         (word_mul
+          (word_sx (word_subword (word_subword zeta (64,64)) (0,32)))
+         (word_sx (word_subword (word_subword h (64,64)) (0,32))))
+        (word_mul (word_sx (word_subword (word_subword zeta (0,64)) (0,32)))
+        (word_sx (word_subword (word_subword h (0,64)) (0,32))))))
+       (128,64))
+      (0,32)))))
+      (word_join
+       (word_mul (word_sx (word_subword (word_subword qinv (64,64)) (0,32)))
+       (word_sx
+       (word_subword
+        (word_subword
+         (word_join
+          (word_join
+           (word_mul
+            (word_sx (word_subword (word_subword zeta (192,64)) (0,32)))
+           (word_sx (word_subword (word_subword h (192,64)) (0,32))))
+          (word_mul
+           (word_sx (word_subword (word_subword zeta (128,64)) (0,32)))
+          (word_sx (word_subword (word_subword h (128,64)) (0,32)))))
+         (word_join
+          (word_mul
+           (word_sx (word_subword (word_subword zeta (64,64)) (0,32)))
+          (word_sx (word_subword (word_subword h (64,64)) (0,32))))
+         (word_mul (word_sx (word_subword (word_subword zeta (0,64)) (0,32)))
+         (word_sx (word_subword (word_subword h (0,64)) (0,32))))))
+        (64,64))
+       (0,32))))
+      (word_mul (word_sx (word_subword (word_subword qinv (0,64)) (0,32)))
+      (word_sx
+      (word_subword
+       (word_subword
+        (word_join
+         (word_join
+          (word_mul
+           (word_sx (word_subword (word_subword zeta (192,64)) (0,32)))
+          (word_sx (word_subword (word_subword h (192,64)) (0,32))))
+         (word_mul
+          (word_sx (word_subword (word_subword zeta (128,64)) (0,32)))
+         (word_sx (word_subword (word_subword h (128,64)) (0,32)))))
+        (word_join
+         (word_mul
+          (word_sx (word_subword (word_subword zeta (64,64)) (0,32)))
+         (word_sx (word_subword (word_subword h (64,64)) (0,32))))
+        (word_mul (word_sx (word_subword (word_subword zeta (0,64)) (0,32)))
+        (word_sx (word_subword (word_subword h (0,64)) (0,32))))))
+       (0,64))
+      (0,32)))))`]
+  2 [`read YMM2 s9 = zeta_high`]
+  3 [`read YMM1 s9 = zeta`]
+  4 [`read YMM0 s9 = qinv`]
+  5 [`read YMM12 s9 =
+      word_join
+      (word_join
+       (word_mul
+        (word_sx (word_subword (word_subword zeta_high (192,64)) (0,32)))
+       (word_sx
+       (word_subword
+        (word_subword
+         (word_join
+          (word_join
+           (word_join (word_subword h (224,32)) (word_subword h (224,32)))
+          (word_join (word_subword h (160,32)) (word_subword h (160,32))))
+         (word_join
+          (word_join (word_subword h (96,32)) (word_subword h (96,32)))
+         (word_join (word_subword h (32,32)) (word_subword h (32,32)))))
+        (192,64))
+       (0,32))))
+      (word_mul
+       (word_sx (word_subword (word_subword zeta_high (128,64)) (0,32)))
+      (word_sx
+      (word_subword
+       (word_subword
+        (word_join
+         (word_join
+          (word_join (word_subword h (224,32)) (word_subword h (224,32)))
+         (word_join (word_subword h (160,32)) (word_subword h (160,32))))
+        (word_join
+         (word_join (word_subword h (96,32)) (word_subword h (96,32)))
+        (word_join (word_subword h (32,32)) (word_subword h (32,32)))))
+       (128,64))
+      (0,32)))))
+      (word_join
+       (word_mul
+        (word_sx (word_subword (word_subword zeta_high (64,64)) (0,32)))
+       (word_sx
+       (word_subword
+        (word_subword
+         (word_join
+          (word_join
+           (word_join (word_subword h (224,32)) (word_subword h (224,32)))
+          (word_join (word_subword h (160,32)) (word_subword h (160,32))))
+         (word_join
+          (word_join (word_subword h (96,32)) (word_subword h (96,32)))
+         (word_join (word_subword h (32,32)) (word_subword h (32,32)))))
+        (64,64))
+       (0,32))))
+      (word_mul
+       (word_sx (word_subword (word_subword zeta_high (0,64)) (0,32)))
+      (word_sx
+      (word_subword
+       (word_subword
+        (word_join
+         (word_join
+          (word_join (word_subword h (224,32)) (word_subword h (224,32)))
+         (word_join (word_subword h (160,32)) (word_subword h (160,32))))
+        (word_join
+         (word_join (word_subword h (96,32)) (word_subword h (96,32)))
+        (word_join (word_subword h (32,32)) (word_subword h (32,32)))))
+       (0,64))
+      (0,32)))))`]
+  6 [`read YMM14 s9 =
+      word_join
+      (word_join
+       (word_mul (word_sx (word_subword (word_subword qinv (192,64)) (0,32)))
+       (word_sx
+       (word_subword
+        (word_subword
+         (word_join
+          (word_join
+           (word_mul
+            (word_sx (word_subword (word_subword zeta (192,64)) (0,32)))
+           (word_sx
+           (word_subword
+            (word_subword
+             (word_join
+              (word_join
+               (word_join (word_subword h (224,32))
+               (word_subword h (224,32)))
+              (word_join (word_subword h (160,32)) (word_subword h (160,32))))
+             (word_join
+              (word_join (word_subword h (96,32)) (word_subword h (96,32)))
+             (word_join (word_subword h (32,32)) (word_subword h (32,32)))))
+            (192,64))
+           (0,32))))
+          (word_mul
+           (word_sx (word_subword (word_subword zeta (128,64)) (0,32)))
+          (word_sx
+          (word_subword
+           (word_subword
+            (word_join
+             (word_join
+              (word_join (word_subword h (224,32)) (word_subword h (224,32)))
+             (word_join (word_subword h (160,32)) (word_subword h (160,32))))
+            (word_join
+             (word_join (word_subword h (96,32)) (word_subword h (96,32)))
+            (word_join (word_subword h (32,32)) (word_subword h (32,32)))))
+           (128,64))
+          (0,32)))))
+         (word_join
+          (word_mul
+           (word_sx (word_subword (word_subword zeta (64,64)) (0,32)))
+          (word_sx
+          (word_subword
+           (word_subword
+            (word_join
+             (word_join
+              (word_join (word_subword h (224,32)) (word_subword h (224,32)))
+             (word_join (word_subword h (160,32)) (word_subword h (160,32))))
+            (word_join
+             (word_join (word_subword h (96,32)) (word_subword h (96,32)))
+            (word_join (word_subword h (32,32)) (word_subword h (32,32)))))
+           (64,64))
+          (0,32))))
+         (word_mul (word_sx (word_subword (word_subword zeta (0,64)) (0,32)))
+         (word_sx
+         (word_subword
+          (word_subword
+           (word_join
+            (word_join
+             (word_join (word_subword h (224,32)) (word_subword h (224,32)))
+            (word_join (word_subword h (160,32)) (word_subword h (160,32))))
+           (word_join
+            (word_join (word_subword h (96,32)) (word_subword h (96,32)))
+           (word_join (word_subword h (32,32)) (word_subword h (32,32)))))
+          (0,64))
+         (0,32))))))
+        (192,64))
+       (0,32))))
+      (word_mul (word_sx (word_subword (word_subword qinv (128,64)) (0,32)))
+      (word_sx
+      (word_subword
+       (word_subword
+        (word_join
+         (word_join
+          (word_mul
+           (word_sx (word_subword (word_subword zeta (192,64)) (0,32)))
+          (word_sx
+          (word_subword
+           (word_subword
+            (word_join
+             (word_join
+              (word_join (word_subword h (224,32)) (word_subword h (224,32)))
+             (word_join (word_subword h (160,32)) (word_subword h (160,32))))
+            (word_join
+             (word_join (word_subword h (96,32)) (word_subword h (96,32)))
+            (word_join (word_subword h (32,32)) (word_subword h (32,32)))))
+           (192,64))
+          (0,32))))
+         (word_mul
+          (word_sx (word_subword (word_subword zeta (128,64)) (0,32)))
+         (word_sx
+         (word_subword
+          (word_subword
+           (word_join
+            (word_join
+             (word_join (word_subword h (224,32)) (word_subword h (224,32)))
+            (word_join (word_subword h (160,32)) (word_subword h (160,32))))
+           (word_join
+            (word_join (word_subword h (96,32)) (word_subword h (96,32)))
+           (word_join (word_subword h (32,32)) (word_subword h (32,32)))))
+          (128,64))
+         (0,32)))))
+        (word_join
+         (word_mul
+          (word_sx (word_subword (word_subword zeta (64,64)) (0,32)))
+         (word_sx
+         (word_subword
+          (word_subword
+           (word_join
+            (word_join
+             (word_join (word_subword h (224,32)) (word_subword h (224,32)))
+            (word_join (word_subword h (160,32)) (word_subword h (160,32))))
+           (word_join
+            (word_join (word_subword h (96,32)) (word_subword h (96,32)))
+           (word_join (word_subword h (32,32)) (word_subword h (32,32)))))
+          (64,64))
+         (0,32))))
+        (word_mul (word_sx (word_subword (word_subword zeta (0,64)) (0,32)))
+        (word_sx
+        (word_subword
+         (word_subword
+          (word_join
+           (word_join
+            (word_join (word_subword h (224,32)) (word_subword h (224,32)))
+           (word_join (word_subword h (160,32)) (word_subword h (160,32))))
+          (word_join
+           (word_join (word_subword h (96,32)) (word_subword h (96,32)))
+          (word_join (word_subword h (32,32)) (word_subword h (32,32)))))
+         (0,64))
+        (0,32))))))
+       (128,64))
+      (0,32)))))
+      (word_join
+       (word_mul (word_sx (word_subword (word_subword qinv (64,64)) (0,32)))
+       (word_sx
+       (word_subword
+        (word_subword
+         (word_join
+          (word_join
+           (word_mul
+            (word_sx (word_subword (word_subword zeta (192,64)) (0,32)))
+           (word_sx
+           (word_subword
+            (word_subword
+             (word_join
+              (word_join
+               (word_join (word_subword h (224,32))
+               (word_subword h (224,32)))
+              (word_join (word_subword h (160,32)) (word_subword h (160,32))))
+             (word_join
+              (word_join (word_subword h (96,32)) (word_subword h (96,32)))
+             (word_join (word_subword h (32,32)) (word_subword h (32,32)))))
+            (192,64))
+           (0,32))))
+          (word_mul
+           (word_sx (word_subword (word_subword zeta (128,64)) (0,32)))
+          (word_sx
+          (word_subword
+           (word_subword
+            (word_join
+             (word_join
+              (word_join (word_subword h (224,32)) (word_subword h (224,32)))
+             (word_join (word_subword h (160,32)) (word_subword h (160,32))))
+            (word_join
+             (word_join (word_subword h (96,32)) (word_subword h (96,32)))
+            (word_join (word_subword h (32,32)) (word_subword h (32,32)))))
+           (128,64))
+          (0,32)))))
+         (word_join
+          (word_mul
+           (word_sx (word_subword (word_subword zeta (64,64)) (0,32)))
+          (word_sx
+          (word_subword
+           (word_subword
+            (word_join
+             (word_join
+              (word_join (word_subword h (224,32)) (word_subword h (224,32)))
+             (word_join (word_subword h (160,32)) (word_subword h (160,32))))
+            (word_join
+             (word_join (word_subword h (96,32)) (word_subword h (96,32)))
+            (word_join (word_subword h (32,32)) (word_subword h (32,32)))))
+           (64,64))
+          (0,32))))
+         (word_mul (word_sx (word_subword (word_subword zeta (0,64)) (0,32)))
+         (word_sx
+         (word_subword
+          (word_subword
+           (word_join
+            (word_join
+             (word_join (word_subword h (224,32)) (word_subword h (224,32)))
+            (word_join (word_subword h (160,32)) (word_subword h (160,32))))
+           (word_join
+            (word_join (word_subword h (96,32)) (word_subword h (96,32)))
+           (word_join (word_subword h (32,32)) (word_subword h (32,32)))))
+          (0,64))
+         (0,32))))))
+        (64,64))
+       (0,32))))
+      (word_mul (word_sx (word_subword (word_subword qinv (0,64)) (0,32)))
+      (word_sx
+      (word_subword
+       (word_subword
+        (word_join
+         (word_join
+          (word_mul
+           (word_sx (word_subword (word_subword zeta (192,64)) (0,32)))
+          (word_sx
+          (word_subword
+           (word_subword
+            (word_join
+             (word_join
+              (word_join (word_subword h (224,32)) (word_subword h (224,32)))
+             (word_join (word_subword h (160,32)) (word_subword h (160,32))))
+            (word_join
+             (word_join (word_subword h (96,32)) (word_subword h (96,32)))
+            (word_join (word_subword h (32,32)) (word_subword h (32,32)))))
+           (192,64))
+          (0,32))))
+         (word_mul
+          (word_sx (word_subword (word_subword zeta (128,64)) (0,32)))
+         (word_sx
+         (word_subword
+          (word_subword
+           (word_join
+            (word_join
+             (word_join (word_subword h (224,32)) (word_subword h (224,32)))
+            (word_join (word_subword h (160,32)) (word_subword h (160,32))))
+           (word_join
+            (word_join (word_subword h (96,32)) (word_subword h (96,32)))
+           (word_join (word_subword h (32,32)) (word_subword h (32,32)))))
+          (128,64))
+         (0,32)))))
+        (word_join
+         (word_mul
+          (word_sx (word_subword (word_subword zeta (64,64)) (0,32)))
+         (word_sx
+         (word_subword
+          (word_subword
+           (word_join
+            (word_join
+             (word_join (word_subword h (224,32)) (word_subword h (224,32)))
+            (word_join (word_subword h (160,32)) (word_subword h (160,32))))
+           (word_join
+            (word_join (word_subword h (96,32)) (word_subword h (96,32)))
+           (word_join (word_subword h (32,32)) (word_subword h (32,32)))))
+          (64,64))
+         (0,32))))
+        (word_mul (word_sx (word_subword (word_subword zeta (0,64)) (0,32)))
+        (word_sx
+        (word_subword
+         (word_subword
+          (word_join
+           (word_join
+            (word_join (word_subword h (224,32)) (word_subword h (224,32)))
+           (word_join (word_subword h (160,32)) (word_subword h (160,32))))
+          (word_join
+           (word_join (word_subword h (96,32)) (word_subword h (96,32)))
+          (word_join (word_subword h (32,32)) (word_subword h (32,32)))))
+         (0,64))
+        (0,32))))))
+       (0,64))
+      (0,32)))))`]
+  7 [`(MAYCHANGE [RIP] ,,
+       MAYCHANGE [YMM13] ,,
+       MAYCHANGE [YMM12] ,,
+       MAYCHANGE [YMM14] ,,
+       MAYCHANGE [YMM8])
+      s0
+      s9`]
+  8 [`read YMM8 s9 =
+      msimd8 (\i x y. if i = word 1 then x else y) (word 170)
+      (word_join
+       (word_join
+        (word_join
+         (word_subword
+          (word_join
+           (word_join
+            (word_mul
+             (word_sx
+             (word_subword (word_subword zeta_high (192,64)) (0,32)))
+            (word_sx (word_subword (word_subword h (192,64)) (0,32))))
+           (word_mul
+            (word_sx (word_subword (word_subword zeta_high (128,64)) (0,32)))
+           (word_sx (word_subword (word_subword h (128,64)) (0,32)))))
+          (word_join
+           (word_mul
+            (word_sx (word_subword (word_subword zeta_high (64,64)) (0,32)))
+           (word_sx (word_subword (word_subword h (64,64)) (0,32))))
+          (word_mul
+           (word_sx (word_subword (word_subword zeta_high (0,64)) (0,32)))
+          (word_sx (word_subword (word_subword h (0,64)) (0,32))))))
+         (224,32))
+        (word_subword
+         (word_join
+          (word_join
+           (word_mul
+            (word_sx (word_subword (word_subword zeta_high (192,64)) (0,32)))
+           (word_sx (word_subword (word_subword h (192,64)) (0,32))))
+          (word_mul
+           (word_sx (word_subword (word_subword zeta_high (128,64)) (0,32)))
+          (word_sx (word_subword (word_subword h (128,64)) (0,32)))))
+         (word_join
+          (word_mul
+           (word_sx (word_subword (word_subword zeta_high (64,64)) (0,32)))
+          (word_sx (word_subword (word_subword h (64,64)) (0,32))))
+         (word_mul
+          (word_sx (word_subword (word_subword zeta_high (0,64)) (0,32)))
+         (word_sx (word_subword (word_subword h (0,64)) (0,32))))))
+        (224,32)))
+       (word_join
+        (word_subword
+         (word_join
+          (word_join
+           (word_mul
+            (word_sx (word_subword (word_subword zeta_high (192,64)) (0,32)))
+           (word_sx (word_subword (word_subword h (192,64)) (0,32))))
+          (word_mul
+           (word_sx (word_subword (word_subword zeta_high (128,64)) (0,32)))
+          (word_sx (word_subword (word_subword h (128,64)) (0,32)))))
+         (word_join
+          (word_mul
+           (word_sx (word_subword (word_subword zeta_high (64,64)) (0,32)))
+          (word_sx (word_subword (word_subword h (64,64)) (0,32))))
+         (word_mul
+          (word_sx (word_subword (word_subword zeta_high (0,64)) (0,32)))
+         (word_sx (word_subword (word_subword h (0,64)) (0,32))))))
+        (160,32))
+       (word_subword
+        (word_join
+         (word_join
+          (word_mul
+           (word_sx (word_subword (word_subword zeta_high (192,64)) (0,32)))
+          (word_sx (word_subword (word_subword h (192,64)) (0,32))))
+         (word_mul
+          (word_sx (word_subword (word_subword zeta_high (128,64)) (0,32)))
+         (word_sx (word_subword (word_subword h (128,64)) (0,32)))))
+        (word_join
+         (word_mul
+          (word_sx (word_subword (word_subword zeta_high (64,64)) (0,32)))
+         (word_sx (word_subword (word_subword h (64,64)) (0,32))))
+        (word_mul
+         (word_sx (word_subword (word_subword zeta_high (0,64)) (0,32)))
+        (word_sx (word_subword (word_subword h (0,64)) (0,32))))))
+       (160,32))))
+      (word_join
+       (word_join
+        (word_subword
+         (word_join
+          (word_join
+           (word_mul
+            (word_sx (word_subword (word_subword zeta_high (192,64)) (0,32)))
+           (word_sx (word_subword (word_subword h (192,64)) (0,32))))
+          (word_mul
+           (word_sx (word_subword (word_subword zeta_high (128,64)) (0,32)))
+          (word_sx (word_subword (word_subword h (128,64)) (0,32)))))
+         (word_join
+          (word_mul
+           (word_sx (word_subword (word_subword zeta_high (64,64)) (0,32)))
+          (word_sx (word_subword (word_subword h (64,64)) (0,32))))
+         (word_mul
+          (word_sx (word_subword (word_subword zeta_high (0,64)) (0,32)))
+         (word_sx (word_subword (word_subword h (0,64)) (0,32))))))
+        (96,32))
+       (word_subword
+        (word_join
+         (word_join
+          (word_mul
+           (word_sx (word_subword (word_subword zeta_high (192,64)) (0,32)))
+          (word_sx (word_subword (word_subword h (192,64)) (0,32))))
+         (word_mul
+          (word_sx (word_subword (word_subword zeta_high (128,64)) (0,32)))
+         (word_sx (word_subword (word_subword h (128,64)) (0,32)))))
+        (word_join
+         (word_mul
+          (word_sx (word_subword (word_subword zeta_high (64,64)) (0,32)))
+         (word_sx (word_subword (word_subword h (64,64)) (0,32))))
+        (word_mul
+         (word_sx (word_subword (word_subword zeta_high (0,64)) (0,32)))
+        (word_sx (word_subword (word_subword h (0,64)) (0,32))))))
+       (96,32)))
+      (word_join
+       (word_subword
+        (word_join
+         (word_join
+          (word_mul
+           (word_sx (word_subword (word_subword zeta_high (192,64)) (0,32)))
+          (word_sx (word_subword (word_subword h (192,64)) (0,32))))
+         (word_mul
+          (word_sx (word_subword (word_subword zeta_high (128,64)) (0,32)))
+         (word_sx (word_subword (word_subword h (128,64)) (0,32)))))
+        (word_join
+         (word_mul
+          (word_sx (word_subword (word_subword zeta_high (64,64)) (0,32)))
+         (word_sx (word_subword (word_subword h (64,64)) (0,32))))
+        (word_mul
+         (word_sx (word_subword (word_subword zeta_high (0,64)) (0,32)))
+        (word_sx (word_subword (word_subword h (0,64)) (0,32))))))
+       (32,32))
+      (word_subword
+       (word_join
+        (word_join
+         (word_mul
+          (word_sx (word_subword (word_subword zeta_high (192,64)) (0,32)))
+         (word_sx (word_subword (word_subword h (192,64)) (0,32))))
+        (word_mul
+         (word_sx (word_subword (word_subword zeta_high (128,64)) (0,32)))
+        (word_sx (word_subword (word_subword h (128,64)) (0,32)))))
+       (word_join
+        (word_mul
+         (word_sx (word_subword (word_subword zeta_high (64,64)) (0,32)))
+        (word_sx (word_subword (word_subword h (64,64)) (0,32))))
+       (word_mul
+        (word_sx (word_subword (word_subword zeta_high (0,64)) (0,32)))
+       (word_sx (word_subword (word_subword h (0,64)) (0,32))))))
+      (32,32)))))
+      (word_join
+       (word_join
+        (word_mul
+         (word_sx (word_subword (word_subword zeta_high (192,64)) (0,32)))
+        (word_sx
+        (word_subword
+         (word_subword
+          (word_join
+           (word_join
+            (word_join (word_subword h (224,32)) (word_subword h (224,32)))
+           (word_join (word_subword h (160,32)) (word_subword h (160,32))))
+          (word_join
+           (word_join (word_subword h (96,32)) (word_subword h (96,32)))
+          (word_join (word_subword h (32,32)) (word_subword h (32,32)))))
+         (192,64))
+        (0,32))))
+       (word_mul
+        (word_sx (word_subword (word_subword zeta_high (128,64)) (0,32)))
+       (word_sx
+       (word_subword
+        (word_subword
+         (word_join
+          (word_join
+           (word_join (word_subword h (224,32)) (word_subword h (224,32)))
+          (word_join (word_subword h (160,32)) (word_subword h (160,32))))
+         (word_join
+          (word_join (word_subword h (96,32)) (word_subword h (96,32)))
+         (word_join (word_subword h (32,32)) (word_subword h (32,32)))))
+        (128,64))
+       (0,32)))))
+      (word_join
+       (word_mul
+        (word_sx (word_subword (word_subword zeta_high (64,64)) (0,32)))
+       (word_sx
+       (word_subword
+        (word_subword
+         (word_join
+          (word_join
+           (word_join (word_subword h (224,32)) (word_subword h (224,32)))
+          (word_join (word_subword h (160,32)) (word_subword h (160,32))))
+         (word_join
+          (word_join (word_subword h (96,32)) (word_subword h (96,32)))
+         (word_join (word_subword h (32,32)) (word_subword h (32,32)))))
+        (64,64))
+       (0,32))))
+      (word_mul
+       (word_sx (word_subword (word_subword zeta_high (0,64)) (0,32)))
+      (word_sx
+      (word_subword
+       (word_subword
+        (word_join
+         (word_join
+          (word_join (word_subword h (224,32)) (word_subword h (224,32)))
+         (word_join (word_subword h (160,32)) (word_subword h (160,32))))
+        (word_join
+         (word_join (word_subword h (96,32)) (word_subword h (96,32)))
+        (word_join (word_subword h (32,32)) (word_subword h (32,32)))))
+       (0,64))
+      (0,32))))))`]
+  9 [`read RIP s9 = word (pc + 46)`]
+
+`eventually x86
+ (\s'.
+      read RIP s' = word (pc + 46) /\
+      (MAYCHANGE [RIP] ,,
+       MAYCHANGE [YMM8; YMM12; YMM13; YMM14] ,,
+       MAYCHANGE [CF; PF; AF; ZF; SF; OF])
+      s0
+      s')
+ s9`
+*)
+
+(* Execute current tatic: ENSURES_FINAL_STATE_TAC *)
+(* Output:
+val it : goalstack = 1 subgoal (1 total)
+
+  0 [`bytes_loaded s9 (word pc) mldsa_mont_mul`]
+  1 [`read YMM13 s9 =
+      word_join
+      (word_join
+       (word_mul (word_sx (word_subword (word_subword qinv (192,64)) (0,32)))
+       (word_sx
+       (word_subword
+        (word_subword
+         (word_join
+          (word_join
+           (word_mul
+            (word_sx (word_subword (word_subword zeta (192,64)) (0,32)))
+           (word_sx (word_subword (word_subword h (192,64)) (0,32))))
+          (word_mul
+           (word_sx (word_subword (word_subword zeta (128,64)) (0,32)))
+          (word_sx (word_subword (word_subword h (128,64)) (0,32)))))
+         (word_join
+          (word_mul
+           (word_sx (word_subword (word_subword zeta (64,64)) (0,32)))
+          (word_sx (word_subword (word_subword h (64,64)) (0,32))))
+         (word_mul (word_sx (word_subword (word_subword zeta (0,64)) (0,32)))
+         (word_sx (word_subword (word_subword h (0,64)) (0,32))))))
+        (192,64))
+       (0,32))))
+      (word_mul (word_sx (word_subword (word_subword qinv (128,64)) (0,32)))
+      (word_sx
+      (word_subword
+       (word_subword
+        (word_join
+         (word_join
+          (word_mul
+           (word_sx (word_subword (word_subword zeta (192,64)) (0,32)))
+          (word_sx (word_subword (word_subword h (192,64)) (0,32))))
+         (word_mul
+          (word_sx (word_subword (word_subword zeta (128,64)) (0,32)))
+         (word_sx (word_subword (word_subword h (128,64)) (0,32)))))
+        (word_join
+         (word_mul
+          (word_sx (word_subword (word_subword zeta (64,64)) (0,32)))
+         (word_sx (word_subword (word_subword h (64,64)) (0,32))))
+        (word_mul (word_sx (word_subword (word_subword zeta (0,64)) (0,32)))
+        (word_sx (word_subword (word_subword h (0,64)) (0,32))))))
+       (128,64))
+      (0,32)))))
+      (word_join
+       (word_mul (word_sx (word_subword (word_subword qinv (64,64)) (0,32)))
+       (word_sx
+       (word_subword
+        (word_subword
+         (word_join
+          (word_join
+           (word_mul
+            (word_sx (word_subword (word_subword zeta (192,64)) (0,32)))
+           (word_sx (word_subword (word_subword h (192,64)) (0,32))))
+          (word_mul
+           (word_sx (word_subword (word_subword zeta (128,64)) (0,32)))
+          (word_sx (word_subword (word_subword h (128,64)) (0,32)))))
+         (word_join
+          (word_mul
+           (word_sx (word_subword (word_subword zeta (64,64)) (0,32)))
+          (word_sx (word_subword (word_subword h (64,64)) (0,32))))
+         (word_mul (word_sx (word_subword (word_subword zeta (0,64)) (0,32)))
+         (word_sx (word_subword (word_subword h (0,64)) (0,32))))))
+        (64,64))
+       (0,32))))
+      (word_mul (word_sx (word_subword (word_subword qinv (0,64)) (0,32)))
+      (word_sx
+      (word_subword
+       (word_subword
+        (word_join
+         (word_join
+          (word_mul
+           (word_sx (word_subword (word_subword zeta (192,64)) (0,32)))
+          (word_sx (word_subword (word_subword h (192,64)) (0,32))))
+         (word_mul
+          (word_sx (word_subword (word_subword zeta (128,64)) (0,32)))
+         (word_sx (word_subword (word_subword h (128,64)) (0,32)))))
+        (word_join
+         (word_mul
+          (word_sx (word_subword (word_subword zeta (64,64)) (0,32)))
+         (word_sx (word_subword (word_subword h (64,64)) (0,32))))
+        (word_mul (word_sx (word_subword (word_subword zeta (0,64)) (0,32)))
+        (word_sx (word_subword (word_subword h (0,64)) (0,32))))))
+       (0,64))
+      (0,32)))))`]
+  2 [`read YMM2 s9 = zeta_high`]
+  3 [`read YMM1 s9 = zeta`]
+  4 [`read YMM0 s9 = qinv`]
+  5 [`read YMM12 s9 =
+      word_join
+      (word_join
+       (word_mul
+        (word_sx (word_subword (word_subword zeta_high (192,64)) (0,32)))
+       (word_sx
+       (word_subword
+        (word_subword
+         (word_join
+          (word_join
+           (word_join (word_subword h (224,32)) (word_subword h (224,32)))
+          (word_join (word_subword h (160,32)) (word_subword h (160,32))))
+         (word_join
+          (word_join (word_subword h (96,32)) (word_subword h (96,32)))
+         (word_join (word_subword h (32,32)) (word_subword h (32,32)))))
+        (192,64))
+       (0,32))))
+      (word_mul
+       (word_sx (word_subword (word_subword zeta_high (128,64)) (0,32)))
+      (word_sx
+      (word_subword
+       (word_subword
+        (word_join
+         (word_join
+          (word_join (word_subword h (224,32)) (word_subword h (224,32)))
+         (word_join (word_subword h (160,32)) (word_subword h (160,32))))
+        (word_join
+         (word_join (word_subword h (96,32)) (word_subword h (96,32)))
+        (word_join (word_subword h (32,32)) (word_subword h (32,32)))))
+       (128,64))
+      (0,32)))))
+      (word_join
+       (word_mul
+        (word_sx (word_subword (word_subword zeta_high (64,64)) (0,32)))
+       (word_sx
+       (word_subword
+        (word_subword
+         (word_join
+          (word_join
+           (word_join (word_subword h (224,32)) (word_subword h (224,32)))
+          (word_join (word_subword h (160,32)) (word_subword h (160,32))))
+         (word_join
+          (word_join (word_subword h (96,32)) (word_subword h (96,32)))
+         (word_join (word_subword h (32,32)) (word_subword h (32,32)))))
+        (64,64))
+       (0,32))))
+      (word_mul
+       (word_sx (word_subword (word_subword zeta_high (0,64)) (0,32)))
+      (word_sx
+      (word_subword
+       (word_subword
+        (word_join
+         (word_join
+          (word_join (word_subword h (224,32)) (word_subword h (224,32)))
+         (word_join (word_subword h (160,32)) (word_subword h (160,32))))
+        (word_join
+         (word_join (word_subword h (96,32)) (word_subword h (96,32)))
+        (word_join (word_subword h (32,32)) (word_subword h (32,32)))))
+       (0,64))
+      (0,32)))))`]
+  6 [`read YMM14 s9 =
+      word_join
+      (word_join
+       (word_mul (word_sx (word_subword (word_subword qinv (192,64)) (0,32)))
+       (word_sx
+       (word_subword
+        (word_subword
+         (word_join
+          (word_join
+           (word_mul
+            (word_sx (word_subword (word_subword zeta (192,64)) (0,32)))
+           (word_sx
+           (word_subword
+            (word_subword
+             (word_join
+              (word_join
+               (word_join (word_subword h (224,32))
+               (word_subword h (224,32)))
+              (word_join (word_subword h (160,32)) (word_subword h (160,32))))
+             (word_join
+              (word_join (word_subword h (96,32)) (word_subword h (96,32)))
+             (word_join (word_subword h (32,32)) (word_subword h (32,32)))))
+            (192,64))
+           (0,32))))
+          (word_mul
+           (word_sx (word_subword (word_subword zeta (128,64)) (0,32)))
+          (word_sx
+          (word_subword
+           (word_subword
+            (word_join
+             (word_join
+              (word_join (word_subword h (224,32)) (word_subword h (224,32)))
+             (word_join (word_subword h (160,32)) (word_subword h (160,32))))
+            (word_join
+             (word_join (word_subword h (96,32)) (word_subword h (96,32)))
+            (word_join (word_subword h (32,32)) (word_subword h (32,32)))))
+           (128,64))
+          (0,32)))))
+         (word_join
+          (word_mul
+           (word_sx (word_subword (word_subword zeta (64,64)) (0,32)))
+          (word_sx
+          (word_subword
+           (word_subword
+            (word_join
+             (word_join
+              (word_join (word_subword h (224,32)) (word_subword h (224,32)))
+             (word_join (word_subword h (160,32)) (word_subword h (160,32))))
+            (word_join
+             (word_join (word_subword h (96,32)) (word_subword h (96,32)))
+            (word_join (word_subword h (32,32)) (word_subword h (32,32)))))
+           (64,64))
+          (0,32))))
+         (word_mul (word_sx (word_subword (word_subword zeta (0,64)) (0,32)))
+         (word_sx
+         (word_subword
+          (word_subword
+           (word_join
+            (word_join
+             (word_join (word_subword h (224,32)) (word_subword h (224,32)))
+            (word_join (word_subword h (160,32)) (word_subword h (160,32))))
+           (word_join
+            (word_join (word_subword h (96,32)) (word_subword h (96,32)))
+           (word_join (word_subword h (32,32)) (word_subword h (32,32)))))
+          (0,64))
+         (0,32))))))
+        (192,64))
+       (0,32))))
+      (word_mul (word_sx (word_subword (word_subword qinv (128,64)) (0,32)))
+      (word_sx
+      (word_subword
+       (word_subword
+        (word_join
+         (word_join
+          (word_mul
+           (word_sx (word_subword (word_subword zeta (192,64)) (0,32)))
+          (word_sx
+          (word_subword
+           (word_subword
+            (word_join
+             (word_join
+              (word_join (word_subword h (224,32)) (word_subword h (224,32)))
+             (word_join (word_subword h (160,32)) (word_subword h (160,32))))
+            (word_join
+             (word_join (word_subword h (96,32)) (word_subword h (96,32)))
+            (word_join (word_subword h (32,32)) (word_subword h (32,32)))))
+           (192,64))
+          (0,32))))
+         (word_mul
+          (word_sx (word_subword (word_subword zeta (128,64)) (0,32)))
+         (word_sx
+         (word_subword
+          (word_subword
+           (word_join
+            (word_join
+             (word_join (word_subword h (224,32)) (word_subword h (224,32)))
+            (word_join (word_subword h (160,32)) (word_subword h (160,32))))
+           (word_join
+            (word_join (word_subword h (96,32)) (word_subword h (96,32)))
+           (word_join (word_subword h (32,32)) (word_subword h (32,32)))))
+          (128,64))
+         (0,32)))))
+        (word_join
+         (word_mul
+          (word_sx (word_subword (word_subword zeta (64,64)) (0,32)))
+         (word_sx
+         (word_subword
+          (word_subword
+           (word_join
+            (word_join
+             (word_join (word_subword h (224,32)) (word_subword h (224,32)))
+            (word_join (word_subword h (160,32)) (word_subword h (160,32))))
+           (word_join
+            (word_join (word_subword h (96,32)) (word_subword h (96,32)))
+           (word_join (word_subword h (32,32)) (word_subword h (32,32)))))
+          (64,64))
+         (0,32))))
+        (word_mul (word_sx (word_subword (word_subword zeta (0,64)) (0,32)))
+        (word_sx
+        (word_subword
+         (word_subword
+          (word_join
+           (word_join
+            (word_join (word_subword h (224,32)) (word_subword h (224,32)))
+           (word_join (word_subword h (160,32)) (word_subword h (160,32))))
+          (word_join
+           (word_join (word_subword h (96,32)) (word_subword h (96,32)))
+          (word_join (word_subword h (32,32)) (word_subword h (32,32)))))
+         (0,64))
+        (0,32))))))
+       (128,64))
+      (0,32)))))
+      (word_join
+       (word_mul (word_sx (word_subword (word_subword qinv (64,64)) (0,32)))
+       (word_sx
+       (word_subword
+        (word_subword
+         (word_join
+          (word_join
+           (word_mul
+            (word_sx (word_subword (word_subword zeta (192,64)) (0,32)))
+           (word_sx
+           (word_subword
+            (word_subword
+             (word_join
+              (word_join
+               (word_join (word_subword h (224,32))
+               (word_subword h (224,32)))
+              (word_join (word_subword h (160,32)) (word_subword h (160,32))))
+             (word_join
+              (word_join (word_subword h (96,32)) (word_subword h (96,32)))
+             (word_join (word_subword h (32,32)) (word_subword h (32,32)))))
+            (192,64))
+           (0,32))))
+          (word_mul
+           (word_sx (word_subword (word_subword zeta (128,64)) (0,32)))
+          (word_sx
+          (word_subword
+           (word_subword
+            (word_join
+             (word_join
+              (word_join (word_subword h (224,32)) (word_subword h (224,32)))
+             (word_join (word_subword h (160,32)) (word_subword h (160,32))))
+            (word_join
+             (word_join (word_subword h (96,32)) (word_subword h (96,32)))
+            (word_join (word_subword h (32,32)) (word_subword h (32,32)))))
+           (128,64))
+          (0,32)))))
+         (word_join
+          (word_mul
+           (word_sx (word_subword (word_subword zeta (64,64)) (0,32)))
+          (word_sx
+          (word_subword
+           (word_subword
+            (word_join
+             (word_join
+              (word_join (word_subword h (224,32)) (word_subword h (224,32)))
+             (word_join (word_subword h (160,32)) (word_subword h (160,32))))
+            (word_join
+             (word_join (word_subword h (96,32)) (word_subword h (96,32)))
+            (word_join (word_subword h (32,32)) (word_subword h (32,32)))))
+           (64,64))
+          (0,32))))
+         (word_mul (word_sx (word_subword (word_subword zeta (0,64)) (0,32)))
+         (word_sx
+         (word_subword
+          (word_subword
+           (word_join
+            (word_join
+             (word_join (word_subword h (224,32)) (word_subword h (224,32)))
+            (word_join (word_subword h (160,32)) (word_subword h (160,32))))
+           (word_join
+            (word_join (word_subword h (96,32)) (word_subword h (96,32)))
+           (word_join (word_subword h (32,32)) (word_subword h (32,32)))))
+          (0,64))
+         (0,32))))))
+        (64,64))
+       (0,32))))
+      (word_mul (word_sx (word_subword (word_subword qinv (0,64)) (0,32)))
+      (word_sx
+      (word_subword
+       (word_subword
+        (word_join
+         (word_join
+          (word_mul
+           (word_sx (word_subword (word_subword zeta (192,64)) (0,32)))
+          (word_sx
+          (word_subword
+           (word_subword
+            (word_join
+             (word_join
+              (word_join (word_subword h (224,32)) (word_subword h (224,32)))
+             (word_join (word_subword h (160,32)) (word_subword h (160,32))))
+            (word_join
+             (word_join (word_subword h (96,32)) (word_subword h (96,32)))
+            (word_join (word_subword h (32,32)) (word_subword h (32,32)))))
+           (192,64))
+          (0,32))))
+         (word_mul
+          (word_sx (word_subword (word_subword zeta (128,64)) (0,32)))
+         (word_sx
+         (word_subword
+          (word_subword
+           (word_join
+            (word_join
+             (word_join (word_subword h (224,32)) (word_subword h (224,32)))
+            (word_join (word_subword h (160,32)) (word_subword h (160,32))))
+           (word_join
+            (word_join (word_subword h (96,32)) (word_subword h (96,32)))
+           (word_join (word_subword h (32,32)) (word_subword h (32,32)))))
+          (128,64))
+         (0,32)))))
+        (word_join
+         (word_mul
+          (word_sx (word_subword (word_subword zeta (64,64)) (0,32)))
+         (word_sx
+         (word_subword
+          (word_subword
+           (word_join
+            (word_join
+             (word_join (word_subword h (224,32)) (word_subword h (224,32)))
+            (word_join (word_subword h (160,32)) (word_subword h (160,32))))
+           (word_join
+            (word_join (word_subword h (96,32)) (word_subword h (96,32)))
+           (word_join (word_subword h (32,32)) (word_subword h (32,32)))))
+          (64,64))
+         (0,32))))
+        (word_mul (word_sx (word_subword (word_subword zeta (0,64)) (0,32)))
+        (word_sx
+        (word_subword
+         (word_subword
+          (word_join
+           (word_join
+            (word_join (word_subword h (224,32)) (word_subword h (224,32)))
+           (word_join (word_subword h (160,32)) (word_subword h (160,32))))
+          (word_join
+           (word_join (word_subword h (96,32)) (word_subword h (96,32)))
+          (word_join (word_subword h (32,32)) (word_subword h (32,32)))))
+         (0,64))
+        (0,32))))))
+       (0,64))
+      (0,32)))))`]
+  7 [`(MAYCHANGE [RIP] ,,
+       MAYCHANGE [YMM13] ,,
+       MAYCHANGE [YMM12] ,,
+       MAYCHANGE [YMM14] ,,
+       MAYCHANGE [YMM8])
+      s0
+      s9`]
+  8 [`read YMM8 s9 =
+      msimd8 (\i x y. if i = word 1 then x else y) (word 170)
+      (word_join
+       (word_join
+        (word_join
+         (word_subword
+          (word_join
+           (word_join
+            (word_mul
+             (word_sx
+             (word_subword (word_subword zeta_high (192,64)) (0,32)))
+            (word_sx (word_subword (word_subword h (192,64)) (0,32))))
+           (word_mul
+            (word_sx (word_subword (word_subword zeta_high (128,64)) (0,32)))
+           (word_sx (word_subword (word_subword h (128,64)) (0,32)))))
+          (word_join
+           (word_mul
+            (word_sx (word_subword (word_subword zeta_high (64,64)) (0,32)))
+           (word_sx (word_subword (word_subword h (64,64)) (0,32))))
+          (word_mul
+           (word_sx (word_subword (word_subword zeta_high (0,64)) (0,32)))
+          (word_sx (word_subword (word_subword h (0,64)) (0,32))))))
+         (224,32))
+        (word_subword
+         (word_join
+          (word_join
+           (word_mul
+            (word_sx (word_subword (word_subword zeta_high (192,64)) (0,32)))
+           (word_sx (word_subword (word_subword h (192,64)) (0,32))))
+          (word_mul
+           (word_sx (word_subword (word_subword zeta_high (128,64)) (0,32)))
+          (word_sx (word_subword (word_subword h (128,64)) (0,32)))))
+         (word_join
+          (word_mul
+           (word_sx (word_subword (word_subword zeta_high (64,64)) (0,32)))
+          (word_sx (word_subword (word_subword h (64,64)) (0,32))))
+         (word_mul
+          (word_sx (word_subword (word_subword zeta_high (0,64)) (0,32)))
+         (word_sx (word_subword (word_subword h (0,64)) (0,32))))))
+        (224,32)))
+       (word_join
+        (word_subword
+         (word_join
+          (word_join
+           (word_mul
+            (word_sx (word_subword (word_subword zeta_high (192,64)) (0,32)))
+           (word_sx (word_subword (word_subword h (192,64)) (0,32))))
+          (word_mul
+           (word_sx (word_subword (word_subword zeta_high (128,64)) (0,32)))
+          (word_sx (word_subword (word_subword h (128,64)) (0,32)))))
+         (word_join
+          (word_mul
+           (word_sx (word_subword (word_subword zeta_high (64,64)) (0,32)))
+          (word_sx (word_subword (word_subword h (64,64)) (0,32))))
+         (word_mul
+          (word_sx (word_subword (word_subword zeta_high (0,64)) (0,32)))
+         (word_sx (word_subword (word_subword h (0,64)) (0,32))))))
+        (160,32))
+       (word_subword
+        (word_join
+         (word_join
+          (word_mul
+           (word_sx (word_subword (word_subword zeta_high (192,64)) (0,32)))
+          (word_sx (word_subword (word_subword h (192,64)) (0,32))))
+         (word_mul
+          (word_sx (word_subword (word_subword zeta_high (128,64)) (0,32)))
+         (word_sx (word_subword (word_subword h (128,64)) (0,32)))))
+        (word_join
+         (word_mul
+          (word_sx (word_subword (word_subword zeta_high (64,64)) (0,32)))
+         (word_sx (word_subword (word_subword h (64,64)) (0,32))))
+        (word_mul
+         (word_sx (word_subword (word_subword zeta_high (0,64)) (0,32)))
+        (word_sx (word_subword (word_subword h (0,64)) (0,32))))))
+       (160,32))))
+      (word_join
+       (word_join
+        (word_subword
+         (word_join
+          (word_join
+           (word_mul
+            (word_sx (word_subword (word_subword zeta_high (192,64)) (0,32)))
+           (word_sx (word_subword (word_subword h (192,64)) (0,32))))
+          (word_mul
+           (word_sx (word_subword (word_subword zeta_high (128,64)) (0,32)))
+          (word_sx (word_subword (word_subword h (128,64)) (0,32)))))
+         (word_join
+          (word_mul
+           (word_sx (word_subword (word_subword zeta_high (64,64)) (0,32)))
+          (word_sx (word_subword (word_subword h (64,64)) (0,32))))
+         (word_mul
+          (word_sx (word_subword (word_subword zeta_high (0,64)) (0,32)))
+         (word_sx (word_subword (word_subword h (0,64)) (0,32))))))
+        (96,32))
+       (word_subword
+        (word_join
+         (word_join
+          (word_mul
+           (word_sx (word_subword (word_subword zeta_high (192,64)) (0,32)))
+          (word_sx (word_subword (word_subword h (192,64)) (0,32))))
+         (word_mul
+          (word_sx (word_subword (word_subword zeta_high (128,64)) (0,32)))
+         (word_sx (word_subword (word_subword h (128,64)) (0,32)))))
+        (word_join
+         (word_mul
+          (word_sx (word_subword (word_subword zeta_high (64,64)) (0,32)))
+         (word_sx (word_subword (word_subword h (64,64)) (0,32))))
+        (word_mul
+         (word_sx (word_subword (word_subword zeta_high (0,64)) (0,32)))
+        (word_sx (word_subword (word_subword h (0,64)) (0,32))))))
+       (96,32)))
+      (word_join
+       (word_subword
+        (word_join
+         (word_join
+          (word_mul
+           (word_sx (word_subword (word_subword zeta_high (192,64)) (0,32)))
+          (word_sx (word_subword (word_subword h (192,64)) (0,32))))
+         (word_mul
+          (word_sx (word_subword (word_subword zeta_high (128,64)) (0,32)))
+         (word_sx (word_subword (word_subword h (128,64)) (0,32)))))
+        (word_join
+         (word_mul
+          (word_sx (word_subword (word_subword zeta_high (64,64)) (0,32)))
+         (word_sx (word_subword (word_subword h (64,64)) (0,32))))
+        (word_mul
+         (word_sx (word_subword (word_subword zeta_high (0,64)) (0,32)))
+        (word_sx (word_subword (word_subword h (0,64)) (0,32))))))
+       (32,32))
+      (word_subword
+       (word_join
+        (word_join
+         (word_mul
+          (word_sx (word_subword (word_subword zeta_high (192,64)) (0,32)))
+         (word_sx (word_subword (word_subword h (192,64)) (0,32))))
+        (word_mul
+         (word_sx (word_subword (word_subword zeta_high (128,64)) (0,32)))
+        (word_sx (word_subword (word_subword h (128,64)) (0,32)))))
+       (word_join
+        (word_mul
+         (word_sx (word_subword (word_subword zeta_high (64,64)) (0,32)))
+        (word_sx (word_subword (word_subword h (64,64)) (0,32))))
+       (word_mul
+        (word_sx (word_subword (word_subword zeta_high (0,64)) (0,32)))
+       (word_sx (word_subword (word_subword h (0,64)) (0,32))))))
+      (32,32)))))
+      (word_join
+       (word_join
+        (word_mul
+         (word_sx (word_subword (word_subword zeta_high (192,64)) (0,32)))
+        (word_sx
+        (word_subword
+         (word_subword
+          (word_join
+           (word_join
+            (word_join (word_subword h (224,32)) (word_subword h (224,32)))
+           (word_join (word_subword h (160,32)) (word_subword h (160,32))))
+          (word_join
+           (word_join (word_subword h (96,32)) (word_subword h (96,32)))
+          (word_join (word_subword h (32,32)) (word_subword h (32,32)))))
+         (192,64))
+        (0,32))))
+       (word_mul
+        (word_sx (word_subword (word_subword zeta_high (128,64)) (0,32)))
+       (word_sx
+       (word_subword
+        (word_subword
+         (word_join
+          (word_join
+           (word_join (word_subword h (224,32)) (word_subword h (224,32)))
+          (word_join (word_subword h (160,32)) (word_subword h (160,32))))
+         (word_join
+          (word_join (word_subword h (96,32)) (word_subword h (96,32)))
+         (word_join (word_subword h (32,32)) (word_subword h (32,32)))))
+        (128,64))
+       (0,32)))))
+      (word_join
+       (word_mul
+        (word_sx (word_subword (word_subword zeta_high (64,64)) (0,32)))
+       (word_sx
+       (word_subword
+        (word_subword
+         (word_join
+          (word_join
+           (word_join (word_subword h (224,32)) (word_subword h (224,32)))
+          (word_join (word_subword h (160,32)) (word_subword h (160,32))))
+         (word_join
+          (word_join (word_subword h (96,32)) (word_subword h (96,32)))
+         (word_join (word_subword h (32,32)) (word_subword h (32,32)))))
+        (64,64))
+       (0,32))))
+      (word_mul
+       (word_sx (word_subword (word_subword zeta_high (0,64)) (0,32)))
+      (word_sx
+      (word_subword
+       (word_subword
+        (word_join
+         (word_join
+          (word_join (word_subword h (224,32)) (word_subword h (224,32)))
+         (word_join (word_subword h (160,32)) (word_subword h (160,32))))
+        (word_join
+         (word_join (word_subword h (96,32)) (word_subword h (96,32)))
+        (word_join (word_subword h (32,32)) (word_subword h (32,32)))))
+       (0,64))
+      (0,32))))))`]
+  9 [`read RIP s9 = word (pc + 46)`]
+
+`read RIP s9 = word (pc + 46) /\
+ (MAYCHANGE [RIP] ,,
+  MAYCHANGE [YMM8; YMM12; YMM13; YMM14] ,,
+  MAYCHANGE [CF; PF; AF; ZF; SF; OF])
+ s0
+ s9`
+*)
+
+(* Execute current tatic: ASM_REWRITE_TAC[] *)
+(* Output:
+val it : goalstack = 1 subgoal (1 total)
+
+  0 [`bytes_loaded s9 (word pc) mldsa_mont_mul`]
+  1 [`read YMM13 s9 =
+      word_join
+      (word_join
+       (word_mul (word_sx (word_subword (word_subword qinv (192,64)) (0,32)))
+       (word_sx
+       (word_subword
+        (word_subword
+         (word_join
+          (word_join
+           (word_mul
+            (word_sx (word_subword (word_subword zeta (192,64)) (0,32)))
+           (word_sx (word_subword (word_subword h (192,64)) (0,32))))
+          (word_mul
+           (word_sx (word_subword (word_subword zeta (128,64)) (0,32)))
+          (word_sx (word_subword (word_subword h (128,64)) (0,32)))))
+         (word_join
+          (word_mul
+           (word_sx (word_subword (word_subword zeta (64,64)) (0,32)))
+          (word_sx (word_subword (word_subword h (64,64)) (0,32))))
+         (word_mul (word_sx (word_subword (word_subword zeta (0,64)) (0,32)))
+         (word_sx (word_subword (word_subword h (0,64)) (0,32))))))
+        (192,64))
+       (0,32))))
+      (word_mul (word_sx (word_subword (word_subword qinv (128,64)) (0,32)))
+      (word_sx
+      (word_subword
+       (word_subword
+        (word_join
+         (word_join
+          (word_mul
+           (word_sx (word_subword (word_subword zeta (192,64)) (0,32)))
+          (word_sx (word_subword (word_subword h (192,64)) (0,32))))
+         (word_mul
+          (word_sx (word_subword (word_subword zeta (128,64)) (0,32)))
+         (word_sx (word_subword (word_subword h (128,64)) (0,32)))))
+        (word_join
+         (word_mul
+          (word_sx (word_subword (word_subword zeta (64,64)) (0,32)))
+         (word_sx (word_subword (word_subword h (64,64)) (0,32))))
+        (word_mul (word_sx (word_subword (word_subword zeta (0,64)) (0,32)))
+        (word_sx (word_subword (word_subword h (0,64)) (0,32))))))
+       (128,64))
+      (0,32)))))
+      (word_join
+       (word_mul (word_sx (word_subword (word_subword qinv (64,64)) (0,32)))
+       (word_sx
+       (word_subword
+        (word_subword
+         (word_join
+          (word_join
+           (word_mul
+            (word_sx (word_subword (word_subword zeta (192,64)) (0,32)))
+           (word_sx (word_subword (word_subword h (192,64)) (0,32))))
+          (word_mul
+           (word_sx (word_subword (word_subword zeta (128,64)) (0,32)))
+          (word_sx (word_subword (word_subword h (128,64)) (0,32)))))
+         (word_join
+          (word_mul
+           (word_sx (word_subword (word_subword zeta (64,64)) (0,32)))
+          (word_sx (word_subword (word_subword h (64,64)) (0,32))))
+         (word_mul (word_sx (word_subword (word_subword zeta (0,64)) (0,32)))
+         (word_sx (word_subword (word_subword h (0,64)) (0,32))))))
+        (64,64))
+       (0,32))))
+      (word_mul (word_sx (word_subword (word_subword qinv (0,64)) (0,32)))
+      (word_sx
+      (word_subword
+       (word_subword
+        (word_join
+         (word_join
+          (word_mul
+           (word_sx (word_subword (word_subword zeta (192,64)) (0,32)))
+          (word_sx (word_subword (word_subword h (192,64)) (0,32))))
+         (word_mul
+          (word_sx (word_subword (word_subword zeta (128,64)) (0,32)))
+         (word_sx (word_subword (word_subword h (128,64)) (0,32)))))
+        (word_join
+         (word_mul
+          (word_sx (word_subword (word_subword zeta (64,64)) (0,32)))
+         (word_sx (word_subword (word_subword h (64,64)) (0,32))))
+        (word_mul (word_sx (word_subword (word_subword zeta (0,64)) (0,32)))
+        (word_sx (word_subword (word_subword h (0,64)) (0,32))))))
+       (0,64))
+      (0,32)))))`]
+  2 [`read YMM2 s9 = zeta_high`]
+  3 [`read YMM1 s9 = zeta`]
+  4 [`read YMM0 s9 = qinv`]
+  5 [`read YMM12 s9 =
+      word_join
+      (word_join
+       (word_mul
+        (word_sx (word_subword (word_subword zeta_high (192,64)) (0,32)))
+       (word_sx
+       (word_subword
+        (word_subword
+         (word_join
+          (word_join
+           (word_join (word_subword h (224,32)) (word_subword h (224,32)))
+          (word_join (word_subword h (160,32)) (word_subword h (160,32))))
+         (word_join
+          (word_join (word_subword h (96,32)) (word_subword h (96,32)))
+         (word_join (word_subword h (32,32)) (word_subword h (32,32)))))
+        (192,64))
+       (0,32))))
+      (word_mul
+       (word_sx (word_subword (word_subword zeta_high (128,64)) (0,32)))
+      (word_sx
+      (word_subword
+       (word_subword
+        (word_join
+         (word_join
+          (word_join (word_subword h (224,32)) (word_subword h (224,32)))
+         (word_join (word_subword h (160,32)) (word_subword h (160,32))))
+        (word_join
+         (word_join (word_subword h (96,32)) (word_subword h (96,32)))
+        (word_join (word_subword h (32,32)) (word_subword h (32,32)))))
+       (128,64))
+      (0,32)))))
+      (word_join
+       (word_mul
+        (word_sx (word_subword (word_subword zeta_high (64,64)) (0,32)))
+       (word_sx
+       (word_subword
+        (word_subword
+         (word_join
+          (word_join
+           (word_join (word_subword h (224,32)) (word_subword h (224,32)))
+          (word_join (word_subword h (160,32)) (word_subword h (160,32))))
+         (word_join
+          (word_join (word_subword h (96,32)) (word_subword h (96,32)))
+         (word_join (word_subword h (32,32)) (word_subword h (32,32)))))
+        (64,64))
+       (0,32))))
+      (word_mul
+       (word_sx (word_subword (word_subword zeta_high (0,64)) (0,32)))
+      (word_sx
+      (word_subword
+       (word_subword
+        (word_join
+         (word_join
+          (word_join (word_subword h (224,32)) (word_subword h (224,32)))
+         (word_join (word_subword h (160,32)) (word_subword h (160,32))))
+        (word_join
+         (word_join (word_subword h (96,32)) (word_subword h (96,32)))
+        (word_join (word_subword h (32,32)) (word_subword h (32,32)))))
+       (0,64))
+      (0,32)))))`]
+  6 [`read YMM14 s9 =
+      word_join
+      (word_join
+       (word_mul (word_sx (word_subword (word_subword qinv (192,64)) (0,32)))
+       (word_sx
+       (word_subword
+        (word_subword
+         (word_join
+          (word_join
+           (word_mul
+            (word_sx (word_subword (word_subword zeta (192,64)) (0,32)))
+           (word_sx
+           (word_subword
+            (word_subword
+             (word_join
+              (word_join
+               (word_join (word_subword h (224,32))
+               (word_subword h (224,32)))
+              (word_join (word_subword h (160,32)) (word_subword h (160,32))))
+             (word_join
+              (word_join (word_subword h (96,32)) (word_subword h (96,32)))
+             (word_join (word_subword h (32,32)) (word_subword h (32,32)))))
+            (192,64))
+           (0,32))))
+          (word_mul
+           (word_sx (word_subword (word_subword zeta (128,64)) (0,32)))
+          (word_sx
+          (word_subword
+           (word_subword
+            (word_join
+             (word_join
+              (word_join (word_subword h (224,32)) (word_subword h (224,32)))
+             (word_join (word_subword h (160,32)) (word_subword h (160,32))))
+            (word_join
+             (word_join (word_subword h (96,32)) (word_subword h (96,32)))
+            (word_join (word_subword h (32,32)) (word_subword h (32,32)))))
+           (128,64))
+          (0,32)))))
+         (word_join
+          (word_mul
+           (word_sx (word_subword (word_subword zeta (64,64)) (0,32)))
+          (word_sx
+          (word_subword
+           (word_subword
+            (word_join
+             (word_join
+              (word_join (word_subword h (224,32)) (word_subword h (224,32)))
+             (word_join (word_subword h (160,32)) (word_subword h (160,32))))
+            (word_join
+             (word_join (word_subword h (96,32)) (word_subword h (96,32)))
+            (word_join (word_subword h (32,32)) (word_subword h (32,32)))))
+           (64,64))
+          (0,32))))
+         (word_mul (word_sx (word_subword (word_subword zeta (0,64)) (0,32)))
+         (word_sx
+         (word_subword
+          (word_subword
+           (word_join
+            (word_join
+             (word_join (word_subword h (224,32)) (word_subword h (224,32)))
+            (word_join (word_subword h (160,32)) (word_subword h (160,32))))
+           (word_join
+            (word_join (word_subword h (96,32)) (word_subword h (96,32)))
+           (word_join (word_subword h (32,32)) (word_subword h (32,32)))))
+          (0,64))
+         (0,32))))))
+        (192,64))
+       (0,32))))
+      (word_mul (word_sx (word_subword (word_subword qinv (128,64)) (0,32)))
+      (word_sx
+      (word_subword
+       (word_subword
+        (word_join
+         (word_join
+          (word_mul
+           (word_sx (word_subword (word_subword zeta (192,64)) (0,32)))
+          (word_sx
+          (word_subword
+           (word_subword
+            (word_join
+             (word_join
+              (word_join (word_subword h (224,32)) (word_subword h (224,32)))
+             (word_join (word_subword h (160,32)) (word_subword h (160,32))))
+            (word_join
+             (word_join (word_subword h (96,32)) (word_subword h (96,32)))
+            (word_join (word_subword h (32,32)) (word_subword h (32,32)))))
+           (192,64))
+          (0,32))))
+         (word_mul
+          (word_sx (word_subword (word_subword zeta (128,64)) (0,32)))
+         (word_sx
+         (word_subword
+          (word_subword
+           (word_join
+            (word_join
+             (word_join (word_subword h (224,32)) (word_subword h (224,32)))
+            (word_join (word_subword h (160,32)) (word_subword h (160,32))))
+           (word_join
+            (word_join (word_subword h (96,32)) (word_subword h (96,32)))
+           (word_join (word_subword h (32,32)) (word_subword h (32,32)))))
+          (128,64))
+         (0,32)))))
+        (word_join
+         (word_mul
+          (word_sx (word_subword (word_subword zeta (64,64)) (0,32)))
+         (word_sx
+         (word_subword
+          (word_subword
+           (word_join
+            (word_join
+             (word_join (word_subword h (224,32)) (word_subword h (224,32)))
+            (word_join (word_subword h (160,32)) (word_subword h (160,32))))
+           (word_join
+            (word_join (word_subword h (96,32)) (word_subword h (96,32)))
+           (word_join (word_subword h (32,32)) (word_subword h (32,32)))))
+          (64,64))
+         (0,32))))
+        (word_mul (word_sx (word_subword (word_subword zeta (0,64)) (0,32)))
+        (word_sx
+        (word_subword
+         (word_subword
+          (word_join
+           (word_join
+            (word_join (word_subword h (224,32)) (word_subword h (224,32)))
+           (word_join (word_subword h (160,32)) (word_subword h (160,32))))
+          (word_join
+           (word_join (word_subword h (96,32)) (word_subword h (96,32)))
+          (word_join (word_subword h (32,32)) (word_subword h (32,32)))))
+         (0,64))
+        (0,32))))))
+       (128,64))
+      (0,32)))))
+      (word_join
+       (word_mul (word_sx (word_subword (word_subword qinv (64,64)) (0,32)))
+       (word_sx
+       (word_subword
+        (word_subword
+         (word_join
+          (word_join
+           (word_mul
+            (word_sx (word_subword (word_subword zeta (192,64)) (0,32)))
+           (word_sx
+           (word_subword
+            (word_subword
+             (word_join
+              (word_join
+               (word_join (word_subword h (224,32))
+               (word_subword h (224,32)))
+              (word_join (word_subword h (160,32)) (word_subword h (160,32))))
+             (word_join
+              (word_join (word_subword h (96,32)) (word_subword h (96,32)))
+             (word_join (word_subword h (32,32)) (word_subword h (32,32)))))
+            (192,64))
+           (0,32))))
+          (word_mul
+           (word_sx (word_subword (word_subword zeta (128,64)) (0,32)))
+          (word_sx
+          (word_subword
+           (word_subword
+            (word_join
+             (word_join
+              (word_join (word_subword h (224,32)) (word_subword h (224,32)))
+             (word_join (word_subword h (160,32)) (word_subword h (160,32))))
+            (word_join
+             (word_join (word_subword h (96,32)) (word_subword h (96,32)))
+            (word_join (word_subword h (32,32)) (word_subword h (32,32)))))
+           (128,64))
+          (0,32)))))
+         (word_join
+          (word_mul
+           (word_sx (word_subword (word_subword zeta (64,64)) (0,32)))
+          (word_sx
+          (word_subword
+           (word_subword
+            (word_join
+             (word_join
+              (word_join (word_subword h (224,32)) (word_subword h (224,32)))
+             (word_join (word_subword h (160,32)) (word_subword h (160,32))))
+            (word_join
+             (word_join (word_subword h (96,32)) (word_subword h (96,32)))
+            (word_join (word_subword h (32,32)) (word_subword h (32,32)))))
+           (64,64))
+          (0,32))))
+         (word_mul (word_sx (word_subword (word_subword zeta (0,64)) (0,32)))
+         (word_sx
+         (word_subword
+          (word_subword
+           (word_join
+            (word_join
+             (word_join (word_subword h (224,32)) (word_subword h (224,32)))
+            (word_join (word_subword h (160,32)) (word_subword h (160,32))))
+           (word_join
+            (word_join (word_subword h (96,32)) (word_subword h (96,32)))
+           (word_join (word_subword h (32,32)) (word_subword h (32,32)))))
+          (0,64))
+         (0,32))))))
+        (64,64))
+       (0,32))))
+      (word_mul (word_sx (word_subword (word_subword qinv (0,64)) (0,32)))
+      (word_sx
+      (word_subword
+       (word_subword
+        (word_join
+         (word_join
+          (word_mul
+           (word_sx (word_subword (word_subword zeta (192,64)) (0,32)))
+          (word_sx
+          (word_subword
+           (word_subword
+            (word_join
+             (word_join
+              (word_join (word_subword h (224,32)) (word_subword h (224,32)))
+             (word_join (word_subword h (160,32)) (word_subword h (160,32))))
+            (word_join
+             (word_join (word_subword h (96,32)) (word_subword h (96,32)))
+            (word_join (word_subword h (32,32)) (word_subword h (32,32)))))
+           (192,64))
+          (0,32))))
+         (word_mul
+          (word_sx (word_subword (word_subword zeta (128,64)) (0,32)))
+         (word_sx
+         (word_subword
+          (word_subword
+           (word_join
+            (word_join
+             (word_join (word_subword h (224,32)) (word_subword h (224,32)))
+            (word_join (word_subword h (160,32)) (word_subword h (160,32))))
+           (word_join
+            (word_join (word_subword h (96,32)) (word_subword h (96,32)))
+           (word_join (word_subword h (32,32)) (word_subword h (32,32)))))
+          (128,64))
+         (0,32)))))
+        (word_join
+         (word_mul
+          (word_sx (word_subword (word_subword zeta (64,64)) (0,32)))
+         (word_sx
+         (word_subword
+          (word_subword
+           (word_join
+            (word_join
+             (word_join (word_subword h (224,32)) (word_subword h (224,32)))
+            (word_join (word_subword h (160,32)) (word_subword h (160,32))))
+           (word_join
+            (word_join (word_subword h (96,32)) (word_subword h (96,32)))
+           (word_join (word_subword h (32,32)) (word_subword h (32,32)))))
+          (64,64))
+         (0,32))))
+        (word_mul (word_sx (word_subword (word_subword zeta (0,64)) (0,32)))
+        (word_sx
+        (word_subword
+         (word_subword
+          (word_join
+           (word_join
+            (word_join (word_subword h (224,32)) (word_subword h (224,32)))
+           (word_join (word_subword h (160,32)) (word_subword h (160,32))))
+          (word_join
+           (word_join (word_subword h (96,32)) (word_subword h (96,32)))
+          (word_join (word_subword h (32,32)) (word_subword h (32,32)))))
+         (0,64))
+        (0,32))))))
+       (0,64))
+      (0,32)))))`]
+  7 [`(MAYCHANGE [RIP] ,,
+       MAYCHANGE [YMM13] ,,
+       MAYCHANGE [YMM12] ,,
+       MAYCHANGE [YMM14] ,,
+       MAYCHANGE [YMM8])
+      s0
+      s9`]
+  8 [`read YMM8 s9 =
+      msimd8 (\i x y. if i = word 1 then x else y) (word 170)
+      (word_join
+       (word_join
+        (word_join
+         (word_subword
+          (word_join
+           (word_join
+            (word_mul
+             (word_sx
+             (word_subword (word_subword zeta_high (192,64)) (0,32)))
+            (word_sx (word_subword (word_subword h (192,64)) (0,32))))
+           (word_mul
+            (word_sx (word_subword (word_subword zeta_high (128,64)) (0,32)))
+           (word_sx (word_subword (word_subword h (128,64)) (0,32)))))
+          (word_join
+           (word_mul
+            (word_sx (word_subword (word_subword zeta_high (64,64)) (0,32)))
+           (word_sx (word_subword (word_subword h (64,64)) (0,32))))
+          (word_mul
+           (word_sx (word_subword (word_subword zeta_high (0,64)) (0,32)))
+          (word_sx (word_subword (word_subword h (0,64)) (0,32))))))
+         (224,32))
+        (word_subword
+         (word_join
+          (word_join
+           (word_mul
+            (word_sx (word_subword (word_subword zeta_high (192,64)) (0,32)))
+           (word_sx (word_subword (word_subword h (192,64)) (0,32))))
+          (word_mul
+           (word_sx (word_subword (word_subword zeta_high (128,64)) (0,32)))
+          (word_sx (word_subword (word_subword h (128,64)) (0,32)))))
+         (word_join
+          (word_mul
+           (word_sx (word_subword (word_subword zeta_high (64,64)) (0,32)))
+          (word_sx (word_subword (word_subword h (64,64)) (0,32))))
+         (word_mul
+          (word_sx (word_subword (word_subword zeta_high (0,64)) (0,32)))
+         (word_sx (word_subword (word_subword h (0,64)) (0,32))))))
+        (224,32)))
+       (word_join
+        (word_subword
+         (word_join
+          (word_join
+           (word_mul
+            (word_sx (word_subword (word_subword zeta_high (192,64)) (0,32)))
+           (word_sx (word_subword (word_subword h (192,64)) (0,32))))
+          (word_mul
+           (word_sx (word_subword (word_subword zeta_high (128,64)) (0,32)))
+          (word_sx (word_subword (word_subword h (128,64)) (0,32)))))
+         (word_join
+          (word_mul
+           (word_sx (word_subword (word_subword zeta_high (64,64)) (0,32)))
+          (word_sx (word_subword (word_subword h (64,64)) (0,32))))
+         (word_mul
+          (word_sx (word_subword (word_subword zeta_high (0,64)) (0,32)))
+         (word_sx (word_subword (word_subword h (0,64)) (0,32))))))
+        (160,32))
+       (word_subword
+        (word_join
+         (word_join
+          (word_mul
+           (word_sx (word_subword (word_subword zeta_high (192,64)) (0,32)))
+          (word_sx (word_subword (word_subword h (192,64)) (0,32))))
+         (word_mul
+          (word_sx (word_subword (word_subword zeta_high (128,64)) (0,32)))
+         (word_sx (word_subword (word_subword h (128,64)) (0,32)))))
+        (word_join
+         (word_mul
+          (word_sx (word_subword (word_subword zeta_high (64,64)) (0,32)))
+         (word_sx (word_subword (word_subword h (64,64)) (0,32))))
+        (word_mul
+         (word_sx (word_subword (word_subword zeta_high (0,64)) (0,32)))
+        (word_sx (word_subword (word_subword h (0,64)) (0,32))))))
+       (160,32))))
+      (word_join
+       (word_join
+        (word_subword
+         (word_join
+          (word_join
+           (word_mul
+            (word_sx (word_subword (word_subword zeta_high (192,64)) (0,32)))
+           (word_sx (word_subword (word_subword h (192,64)) (0,32))))
+          (word_mul
+           (word_sx (word_subword (word_subword zeta_high (128,64)) (0,32)))
+          (word_sx (word_subword (word_subword h (128,64)) (0,32)))))
+         (word_join
+          (word_mul
+           (word_sx (word_subword (word_subword zeta_high (64,64)) (0,32)))
+          (word_sx (word_subword (word_subword h (64,64)) (0,32))))
+         (word_mul
+          (word_sx (word_subword (word_subword zeta_high (0,64)) (0,32)))
+         (word_sx (word_subword (word_subword h (0,64)) (0,32))))))
+        (96,32))
+       (word_subword
+        (word_join
+         (word_join
+          (word_mul
+           (word_sx (word_subword (word_subword zeta_high (192,64)) (0,32)))
+          (word_sx (word_subword (word_subword h (192,64)) (0,32))))
+         (word_mul
+          (word_sx (word_subword (word_subword zeta_high (128,64)) (0,32)))
+         (word_sx (word_subword (word_subword h (128,64)) (0,32)))))
+        (word_join
+         (word_mul
+          (word_sx (word_subword (word_subword zeta_high (64,64)) (0,32)))
+         (word_sx (word_subword (word_subword h (64,64)) (0,32))))
+        (word_mul
+         (word_sx (word_subword (word_subword zeta_high (0,64)) (0,32)))
+        (word_sx (word_subword (word_subword h (0,64)) (0,32))))))
+       (96,32)))
+      (word_join
+       (word_subword
+        (word_join
+         (word_join
+          (word_mul
+           (word_sx (word_subword (word_subword zeta_high (192,64)) (0,32)))
+          (word_sx (word_subword (word_subword h (192,64)) (0,32))))
+         (word_mul
+          (word_sx (word_subword (word_subword zeta_high (128,64)) (0,32)))
+         (word_sx (word_subword (word_subword h (128,64)) (0,32)))))
+        (word_join
+         (word_mul
+          (word_sx (word_subword (word_subword zeta_high (64,64)) (0,32)))
+         (word_sx (word_subword (word_subword h (64,64)) (0,32))))
+        (word_mul
+         (word_sx (word_subword (word_subword zeta_high (0,64)) (0,32)))
+        (word_sx (word_subword (word_subword h (0,64)) (0,32))))))
+       (32,32))
+      (word_subword
+       (word_join
+        (word_join
+         (word_mul
+          (word_sx (word_subword (word_subword zeta_high (192,64)) (0,32)))
+         (word_sx (word_subword (word_subword h (192,64)) (0,32))))
+        (word_mul
+         (word_sx (word_subword (word_subword zeta_high (128,64)) (0,32)))
+        (word_sx (word_subword (word_subword h (128,64)) (0,32)))))
+       (word_join
+        (word_mul
+         (word_sx (word_subword (word_subword zeta_high (64,64)) (0,32)))
+        (word_sx (word_subword (word_subword h (64,64)) (0,32))))
+       (word_mul
+        (word_sx (word_subword (word_subword zeta_high (0,64)) (0,32)))
+       (word_sx (word_subword (word_subword h (0,64)) (0,32))))))
+      (32,32)))))
+      (word_join
+       (word_join
+        (word_mul
+         (word_sx (word_subword (word_subword zeta_high (192,64)) (0,32)))
+        (word_sx
+        (word_subword
+         (word_subword
+          (word_join
+           (word_join
+            (word_join (word_subword h (224,32)) (word_subword h (224,32)))
+           (word_join (word_subword h (160,32)) (word_subword h (160,32))))
+          (word_join
+           (word_join (word_subword h (96,32)) (word_subword h (96,32)))
+          (word_join (word_subword h (32,32)) (word_subword h (32,32)))))
+         (192,64))
+        (0,32))))
+       (word_mul
+        (word_sx (word_subword (word_subword zeta_high (128,64)) (0,32)))
+       (word_sx
+       (word_subword
+        (word_subword
+         (word_join
+          (word_join
+           (word_join (word_subword h (224,32)) (word_subword h (224,32)))
+          (word_join (word_subword h (160,32)) (word_subword h (160,32))))
+         (word_join
+          (word_join (word_subword h (96,32)) (word_subword h (96,32)))
+         (word_join (word_subword h (32,32)) (word_subword h (32,32)))))
+        (128,64))
+       (0,32)))))
+      (word_join
+       (word_mul
+        (word_sx (word_subword (word_subword zeta_high (64,64)) (0,32)))
+       (word_sx
+       (word_subword
+        (word_subword
+         (word_join
+          (word_join
+           (word_join (word_subword h (224,32)) (word_subword h (224,32)))
+          (word_join (word_subword h (160,32)) (word_subword h (160,32))))
+         (word_join
+          (word_join (word_subword h (96,32)) (word_subword h (96,32)))
+         (word_join (word_subword h (32,32)) (word_subword h (32,32)))))
+        (64,64))
+       (0,32))))
+      (word_mul
+       (word_sx (word_subword (word_subword zeta_high (0,64)) (0,32)))
+      (word_sx
+      (word_subword
+       (word_subword
+        (word_join
+         (word_join
+          (word_join (word_subword h (224,32)) (word_subword h (224,32)))
+         (word_join (word_subword h (160,32)) (word_subword h (160,32))))
+        (word_join
+         (word_join (word_subword h (96,32)) (word_subword h (96,32)))
+        (word_join (word_subword h (32,32)) (word_subword h (32,32)))))
+       (0,64))
+      (0,32))))))`]
+  9 [`read RIP s9 = word (pc + 46)`]
+
+`(MAYCHANGE [RIP] ,,
+  MAYCHANGE [YMM8; YMM12; YMM13; YMM14] ,,
+  MAYCHANGE [CF; PF; AF; ZF; SF; OF])
+ s0
+ s9`
+*)
